\documentclass[10pt, a4paper, twocolumn]{article}
\usepackage[margin=0.3cm]{geometry}
\usepackage{amsfonts, amsmath, amssymb, bm, extarrows}
%\usepackage[none]{hyphenat}%prevent hyphenated words
\usepackage{fancyhdr}
\usepackage{graphicx, float}
%\usepackage{multicol}
\usepackage{multirow}
\usepackage{siunitx}

\allowdisplaybreaks%允许公式换页

\def\D{\partial}
\def\d{\,\mathrm{d}}
\def\epsilon{\varepsilon}
\def\Phi{\varPhi}
\def\phi{\varphi}
\def\Res{\mathrm{Res}}
\def\F{\mathfrak{F}}
\def\L{\mathfrak{L}}

% opening
% \title{Solving PDEs - MMP Final Prep}
% \author{He Yujie}

\begin{document}

\section{Basic PDEs}
\subsection{Classification and transformation of eqs}

	\begin{align*}
		&a_{11}u_{xx} + 2a_{12}u_{xy} + a_{22}u_{yy} + b_1u_x + b_2u_y + cu + f = 0\\
		&a_{11}\left(\d y/\d x\right)^2 - 2a_{12}\d y/\d x + a_{22} = 0, \Delta = a_{12}^2 - a_{11}a_{22}\\
		&A_{11}u_{\xi\xi} + 2A_{12}u_{\xi\eta} + A_{22}u_{\eta\eta} + B_1u_\xi + B_2u_\eta + Cu + F = 0\\
		&\left\{\begin{aligned}
			&A_{11} = a_{11}\xi_x^2 + 2a_{12}\xi_x\xi_y + a_{22}\xi_y^2\\
			&A_{12} = a_{11}\xi_x\eta_x + a_{12}(\xi_x\eta_y+\xi_y\eta_y)+a_22\xi_y\eta_y\\
			&A_{22} = a_{11}\eta_x^2 + 2a_{12}\eta_x\eta_y + a_{22}\eta_y^2\\
			&B_1=a_{11}\xi_{xx} + 2a_{12}\xi_{xy} + a_{22}\xi_{yy} + b_1\xi{yy}
			+b_1\xi_x + b_2\xi_y\\
			&B_2=a_{11}\eta_{xx} + 2a_{12}\eta_{xy} + a_{22}\eta_{yy} + b_1\eta{yy}
			+b_1\eta_x + b_2\eta_y\\
			&C=c\\
			&F=f
		\end{aligned}\right.\\
		&\text{Hyperbolic eqs. } (\Delta > 0)\\
		&u_{\rho\rho} - u_{\sigma\sigma} + \dfrac{1}{2A_{12}}
			((B_1+B_2)u_\rho + (B_1-B_2)u_\sigma + Cu + F) = 0\\
		&\left\{\begin{aligned}
			&\rho = \xi + \eta\\
			&\sigma = \xi - \eta
		\end{aligned}\right.\\
		&\text{Parabolic eqs. } (\Delta = 0)\\
		&u_{\eta\eta} + \dfrac{1}{A_{22}}
			(B_1u_\xi + B_2u_\eta + Cu + F) = 0\\
		&\text{Elliptic eqs. } (\Delta < 0)\\
		&u_{\rho\rho} + u_{\sigma\sigma} + \dfrac{1}{2A_{12}}
			((B_1+B_2)u_\rho + i(B_1-B_2)u_\sigma + Cu + F) = 0\\
		&\left\{\begin{aligned}
			&\rho = \xi + \eta\\
			&\sigma = i(\xi - \eta)
		\end{aligned}\right.\\
		&\text{append.}\left\{\begin{aligned}
			&u_\xi = u_\rho + (i)u_\sigma\\
			&u_\eta = u_\rho - (i)u_\sigma\\
			&u_{\xi\eta} = u_{\rho\rho} -(i^2) u_{\sigma\sigma}
		\end{aligned}\right.\\
	\end{align*}

\subsection{Traveling wave method}

	\begin{align*}
		&u_{tt} - a^2u_{xx}=0, u|_{t=0} = \phi(x), u_t|_{t=0} = \psi(x), (-\infty<x<\infty)\\
		&u(x,t) = \dfrac{1}{2}[\phi(x+at)+\phi(x-at)] + \dfrac{1}{2a}
		\int\limits^{x+at}_{x-at}\psi(\xi)\d\xi
	\end{align*}

\subsection{Wave eq and Transport eqs}

	Nonhomogeneous boundary condition: use superstition principle(twice) to 
	simplify a general problem to 3 part: 1 known, 1 with nonhomogeneous initial 
	condition and 1 with nonhomogeneous equation.
	Nonhomogeneous equation: impulse theorem method or Fourier series method.

\subsection{Steady Field Problems}

	Nonhomogeneous equation: use superstition principle(twice) to 
	simplify a general problem to 3 part: 1 known particular solution, 2 with 
	one nonhomogeneous boundary problem.

	2-D round Laplace eq $$u(\rho, \phi) = C_0 + D_0\ln\rho + \sum^\infty_{n=1}
		(A_n\cos m\phi + B_n\sin m\phi)(C_m\rho^m + D_m\rho^{-m})$$
	2-D Laplace eq $$ u(x, y) = C_0 + \sum^\infty_{n=1}(A_n e^{\frac{n \pi y}{a}} + 
		B_n e^{-\frac{n \pi y}{a}})(C_n\cos\dfrac{n\pi}{a}x + D_n \sin\dfrac{n\pi}{a}x)$$

\section{Special PDEs}
	\begin{align*}
		\Delta u &= \dfrac{1}{\rho}\dfrac{\D}{\D\rho}
			\left(\rho\dfrac{\D u}{\D\rho}\right)
			+ \dfrac{1}{\rho^2}\dfrac{\D^2u}{\D\phi^2}\\
		&= \dfrac{\D^2u}{\D\rho^2}
			+ \dfrac{1}{\rho}\dfrac{\D u}{\D\rho}
			+ \dfrac{1}{\rho^2}\dfrac{\D^2u}{\D\phi^2}\\
		\Delta u &= \dfrac{1}{r^2}\dfrac{\D}{\D r}\left(r^2\dfrac{\D u}{\D r}\right)
			+ \dfrac{1}{r^2\sin\theta}\dfrac{\D}{\D\theta}
			\left(\sin\theta\dfrac{\D u}{\D\theta}\right)
			+ \dfrac{1}{r^2\sin^2\theta}\dfrac{\D^2u}{\D\phi^2}
	\end{align*}

	% \begin{figure}[h!]
	% 	\centering
	% 	\includegraphics[width=\linewidth]{Table2.png}
	% \end{figure}

\subsection{About Ordinary Point}

	standard form: $\dfrac{\d^2w}{\d z^2} + p(z)\dfrac{\d w}{\d x} + q(z)w = 0$, 
	$w(z_0)=C_0$, $w'(z_0)=C_1$. If $p(z), q(z)$ analytic in $|z-z_0|<R$(ordinary 
	point), then solution is unique and
	$$w(z) = \sum^\infty_{k=0}a_k(z-z_0)^k, |z-z_0|<R$$

\subsection{About Regular Singular Point}

	If $(z-z_0)p(z), (z-z_0)^2q(z)$ analytic in $|z-z_0|<R$ ($z_0$ is at most 1st 
	order singular point of $p(z)$, 2nd order singular point of $q(z)$, regular 
	singular point), then there are 2 regular sulution(linear independent and 
	with finite negative power terms):
	\begin{align*}
		&w_1(z) = \sum^\infty_{-\infty}a_k(z-z_0)^{s_1+k}\\
		&w_2(z) = \sum^\infty_{-\infty}b_k(z-z_0)^{s_2+k}\\
		\text{or}\quad &w_2(z) = Aw_1(z)\ln(z-z_0) + \sum^\infty_{-\infty}b_k(z-z_0)^{s_2+k}
	\end{align*}
	Where $s_1, s_2$: $s(s-1) + sp_{-1} + q_{-2} = 0 $

\section{Spherical Functions}
	\begin{align*}
		u(r,\theta,\phi) = \sum_{m=0}^\infty\sum_{l=m}^\infty r^l(A^m_l\cos m\phi + B^m_l\sin m\phi)P^m_l(\cos\theta)\\
		+ \sum_{m=0}^\infty\sum_{l=m}^\infty \dfrac{1}{r^{l+1}}(C^m_l\cos m\phi + D^m_l\sin m\phi)P^m_l(\cos\theta)
	\end{align*}

\subsection{Legendre Eqs (m=0)}
	\begin{align*}
		&P_l(x) = \dfrac{1}{2^ll!}\dfrac{\d^l}{\d x^l}(x^2-1)^l\\
		&a_k = \dfrac{(k+2)(k+1)}{(k-l)(k+l+1)}a_{k+2}, \quad a_l = \dfrac{(2l)!}{2^ll!}\\
		&P_{2n}(0) = (-1)^n \dfrac{(2n-1)!!}{(2n)!!}, \quad P_l(1) = 1\\
		&\dfrac{1}{d} = \dfrac{1}{\sqrt{R^2 - 2rR\cos\theta + r^2}}
			=\left\{\begin{aligned}
				&\sum^\infty_{l=0}\dfrac{r^l}{R^{l+1}}P_l(\cos\theta), r<R\\
				&\sum^\infty_{l=0}\dfrac{R^l}{r^{l+1}}P_l(\cos\theta), r>R
			\end{aligned}\right.
	\end{align*}
	Fourier expansion $f(x) = \displaystyle\sum^\infty_{l=0}f_lP_l(x), \quad -1 \leq x \leq 1$
	
	where $f_l = \dfrac{1}{N_l^2}\displaystyle\int \limits^1_{-1}f(x)P_l(x)\d x, N_l^2 = \dfrac{2}{2l+1}$
	
	Recurrence formula for Legendre Polynomial
	\begin{align*}
		(k+1)P_{k+1}(X) &= (2k+1)xP_k(x) - kP_{k-1}(x) 0, (k\geq 1)\\
		(2k+1)P_k(x) &= P'_{k+1}(x) - P'_{k-1}(x), (k\geq 1)\\
		P'_{k+1}(x) &= (k+1)P_k(x) + xP'_k(x)\\
		kP_k(x) &= xP'_k(x) - P'_{k-1}(x), (k\geq 1)\\
		(x^2 -1)P'_k(x) &= kxP_k(x) - kP_{k-1}(x), (k\geq 1)
	\end{align*}
	Legendre Polynomial
	\begin{align*}
		&P_0(x) = 1\\
		&P_1(x) = x = \cos\theta\\
		&P_2(x) = \dfrac{1}{2}(3x^2 - 1) = \dfrac{1}{4}(3\cos2\theta + 1)\\
		&P_3(x) = \dfrac{1}{8}(35x^4 - 30x^2 + 3)
				= \dfrac{1}{64}(35\cos4\theta + 20\cos2\theta + 9)
	\end{align*}
	
\subsection{Associated Legendre Eqs}
	Basics
	\begin{align*}
		&P_l^m(x) = (1-x^2)^{\frac{m}{2}}P^{(m)}_l(x), \text{with fixed m, l from 0 to m}\\
		&P_l^m(x) = \dfrac{(1-x^2)^{\frac{m}{2}}}{2^l l!}\dfrac{\d^{l+m}}{\d x^{l+m}}(x^2-1)^l\\
	\end{align*}
	Fourier expansion $f(x) = \displaystyle\sum^\infty_{l=m}f_lP^m_l(x), \quad -1 \leq x \leq 1$
	
	where $f_l = \dfrac{1}{(N^m_l)^2}\displaystyle\int \limits^1_{-1}f(x)P^m_l(x)\d x, [N^m_l]^2 = \dfrac{2}{2l+1}\dfrac{(l+m)!}{(l-m)!}$
	
	Associated Legendre Polynomial
	\begin{align*}
		P^1_1(x) &= (1-x^2)^{\frac{1}{2}}=\sin\theta\\
		P^1_2(x) &= 3(1-x^2)^{\frac{1}{2}}x = \dfrac{3}{2}\sin2\theta = 3\sin\theta\cos\theta\\
		P^1_3(x) &= \dfrac{3}{2}(1-x^2)^{\frac{1}{2}}(5x^2-1) = \dfrac{3}{8}(\sin\theta+5\sin3\theta)\\
		&= 6\sin\theta - \dfrac{15}{2}\sin^3\theta\\
		P^2_2(x) &= 3(1-x^2) = \dfrac{3}{2}(1-\cos2\theta) = 3\sin^2\theta\\
		P^2_3(x) &= 15(1-x^2)x = \dfrac{15}{4}(\cos\theta-\cos3\theta) = 15\sin^2\theta\cos\theta\\
		P^3_3(x) &= 15(1-x^2)^{\frac{3}{2}}=\dfrac{15}{4}(3\sin\theta-\sin3\theta) = 15\sin^3\theta
	\end{align*}

\subsection{General Spherical Functions}

	\begin{align*}
		&Y^m_l(\theta,\phi) = P^{|m|}_l(\cos\theta)e^{im\phi}\\
		&[N^m_l]^2 = \dfrac{4\pi}{2l+1}\dfrac{(l+|m|)!}{(l-|m|)!}
	\end{align*}
	Fourier expansion
	$$f(\theta, \phi) =g(\theta)h(\phi) = \displaystyle\sum^\infty_{l=0}\sum^l_{m=-l}C^m_lP^{|m|}_l(\cos\theta)e^{im\phi}$$
	$$C^m_l = \dfrac{1}{[N^m_l]^2}\displaystyle\int \limits^\pi_{0}g(\theta)P^m_l(\cos\theta)\sin\theta\d \theta
		\int\limits^{2\pi}_0 h(\phi)e^{-im\phi}\d \phi$$

\section{Cylinder Functions}
	Differentiation and integrals (for Bessel and Neumann functions)
	
	\begin{align*}
		x^{-\nu} J_{\nu+1}(x)\d x &= -\d \left(x^{-\nu} J_\nu(x)\right)\\
		x^\nu J_{\nu-1}(x)\d x &= \d \left(x^\nu J_\nu(x)\right)\\
		J_1(x)\d x &= -\d (J_0(x))
	\end{align*}
	Recurrence formula for Cylinder functions
	\begin{align*}
		&Z'_\nu(x) - \nu x^{-1}Z_\nu(x) = -Z_{\nu+1}(x)\\
		&Z'_\nu(x) + \nu x^{-1}Z_\nu(x) = Z_{\nu-1}(x)\\
		&Z_{\nu-1}(x) - Z_{\nu+1}(x) = 2Z'_\nu(x)\\
		&Z_{\nu+1}(x) - 2\nu x^{-1} Z_\nu(x) + Z_{\nu-1}(x) = 0
	\end{align*}

\subsection{Bessel Function}

% If boundary condition is homogeneous on the side($R(\rho)$), consider $\mu\geq 0$.
	\begin{align*}
		&x^2\dfrac{\d^2 R}{\d r^2} + 2r\dfrac{\d R}{\d r} + (x^2 - m^2)R=0\\
		&J_\nu(x) = \sum^\infty_{k=0}(-1)^k\dfrac{1}{k!\Gamma(\nu+k+1)}\left(\dfrac{x}{2}\right)^{\nu+2k}\\
		&x\rightarrow 0: J_0(x)\rightarrow 1, J_\nu(x) \rightarrow 0, J_{-\nu}(x) \rightarrow \infty\\
		&x\rightarrow \infty: J_{\pm\nu}(x)\rightarrow 0, N_\nu(x)\rightarrow 0
	\end{align*}
	% Eigenvalue problems (formally denoted) dependent on BC
	% \footnote{especially, $x^{(0,2)}_n = x^{(1,1)}_n$ for $J'_0(x) = -J_1(x)$}
	% \begin{align*}
	% 	&\mu^{(m,1)}_n = (x^{(m,1)}_n/\rho_0)^2, &J_m(\sqrt{\mu}\rho_0)=0\\
	% 	&\mu^{(m,2)}_n = (x^{(m,2)}_n/\rho_0)^2, &J'_m(\sqrt{\mu}\rho_0)=0\\
	% 	&\mu^{(m,3)}_n = (x^{(m,3)}_n/\rho_0)^2, &J_m + H\sqrt{\mu}J'_m=0
	% \end{align*}
	Fourier expansion $f(\rho) = \displaystyle\sum^\infty_{n=1}f_nJ_m(\sqrt{\mu}\rho), 
		\quad 0 \leq \rho \leq \rho_0$
	
	where $f_n = \dfrac{1}{[N^{(m)}_n]^2}\displaystyle\int \limits^{\rho_0}_{0}
		f(\rho)J_m(\sqrt{\mu}\rho)\rho\d \rho$, $f_0 = 
		\dfrac{2}{\rho_0^2}\displaystyle\int\limits^{\rho_0}_0f(\rho)\rho\d \rho$
	
	Norm of Bessel function dependent on BC
	\begin{align*}
		&[N^{(m)}_n]^2 = \dfrac{1}{2} \rho^2_0 [J_{m+1}(\sqrt{\mu^{(m)}_n}\rho_0)]^2,\quad J_m(\sqrt{\mu}\rho_0)=0\\
		&[N^{(m)}_n]^2 = \dfrac{1}{2}\left(\rho_0^2 - \dfrac{m^2}{\mu^{(m)}_n}\right)
			[J_{m}(\sqrt{\mu^{(m)}_n}\rho_0)]^2,\quad J'_m(\sqrt{\mu}\rho_0)=0\\
		&[N^{(m)}_n]^2 = \dfrac{1}{2}\left(\rho_0^2 - \dfrac{m^2}{\mu^{(m)}_n} + \dfrac{\rho^2_0}{H\mu^{(m)}_n}\right)
			[J_{m}(\sqrt{\mu^{(m)}_n}\rho_0)]^2,\\ 
			&\qquad\qquad\qquad\qquad\qquad\qquad\qquad\qquad\qquad\quad J_m + H\sqrt{\mu}J'_m=0
	\end{align*}

\subsection{Bessel Function of Imaginary Argument}

	% If boundary condition is homogeneous for upper and lower surface($Z(z)$)
	% and nonhomogeneous on the side($R(\rho)$), consider $\mu\leq 0$.
	\begin{align*}
		&x^2\dfrac{\d^2 R}{\d r^2} + 2r\dfrac{\d R}{\d r} - (x^2 + m^2)R=0\\
		&I_m(x)=\sum^\infty_{k=0}\dfrac{1}{k!(m+k)!}\left(\dfrac{x}{2}\right)^{m+2k}\\
		&x\rightarrow 0: I_0(x)\rightarrow 1, I_m(x) \rightarrow 0, K_m(x) \rightarrow \infty\\
		&x\rightarrow \infty: I_m(x)\rightarrow \infty, K_m(x)\rightarrow 0
	\end{align*}

\subsection{Spherical Bessel Function}

	\begin{align*}
		&r^2\dfrac{\d R}{\d r^2} + 2r\dfrac{\d R}{\d r} + [k^2r^2-(l+1)]R=0\\
		&j_l(x) = \sqrt{\dfrac{\pi}{2x}}J_{l+\frac{1}{2}}(x), n_l(x) = \sqrt{\dfrac{\pi}{2x}}N_{l+\frac{1}{2}}(x),\\
		&x\rightarrow 0: j_0(x)\rightarrow 1, j_l(x)\rightarrow 0, n_{l}(x) \rightarrow \infty\\
		&x\rightarrow \infty: j_l(x)\rightarrow 0, n_{l}(x) \rightarrow 0
	\end{align*}
	Fourier expansion $f(r) = \displaystyle\sum^\infty_{m=1}f_mj_l(k_m r), 0 \leq r \leq r_0$
	$$f_m = \dfrac{1}{[N_m]^2} \displaystyle\int \limits^{r_0}_0 f(r)j_l(k_m r)r^2\d r$$
	$$[N_m]^2 = \int^{r_0}_0 [j_l(k_m r)]^2 r^2 \d r$$
	
	Spherical Bessel function
	\begin{align*}
		&j_0(x) = \dfrac{\sin x}{x}\\
		&j_1(x) = \dfrac{1}{x^2}(\sin x - x\cos x)\\
		&j_2(x) = \dfrac{1}{x^3}[3(\sin x - x\cos x)-x^2\sin x]\\
		&n_0(x) = -\dfrac{1}{x}\cos x\\
		&n_1(x) = -\dfrac{1}{x^2}(\cos x + x\sin x)\\
		&n_2(x) = -\dfrac{1}{x^3}[3(\cos x + x\sin x) - x^2\cos x]
	\end{align*}
\section{Green Function Method}
	1st Green formula $$\iint\limits_\Sigma u\nabla v\cdot \d\bm{s}
		= \iiint \limits_T \nabla \cdot (u \nabla v) \d V
		= \iiint \limits_T u \Delta v \d V
		+ \iiint \limits_T \nabla v \cdot \nabla v \d V$$
	2nd Green formula $$\iint \limits_\Sigma (u \nabla v - v \nabla u) \d\bm{s}
		= \iiint \limits_T (u \Delta v - v \Delta u) \d V$$
	$$\iint \limits_\Sigma \left(u\dfrac{\D v}{\D n} - v\dfrac{\D u}{\D n}\right)\d s
	= \iiint \limits_T (u \Delta v - v \Delta u) \d V$$
	Poisson problem
	\begin{align*}
		\left\{\begin{aligned}
		&\Delta u(\bm{r}) = f(\bm{r})\\
		&\left.\left(\alpha \dfrac{\D u}{\D n} + \beta u \right)\right|_\Sigma = \phi(\bm{r})
		\end{aligned}\right.
	\end{align*}
	Solution with Green function
	\begin{align*}
		&u(\bm{r_0}) = \iiint \limits_T v(\bm{r}, \bm{r}_0)f(\bm{r})\d V
			- \iint \limits_\Sigma\left(v(\bm{r}, \bm{r}_0) \dfrac{\D u(\bm{r})}{\D n}
			- u(\bm{r}) \dfrac{\D v(\bm{r}, \bm{r}_0)}{\D n}\right)\d S\\
		&u(\bm{r_0}) = \iiint \limits_T G(\bm{r}, \bm{r}_0)f(\bm{r})\d V
			+ \iint \limits_\Sigma \phi(\bm{r}) \dfrac{\D G(\bm{r}, \bm{r}_0)}{\D n}\d S\\
		&u(\bm{r_0}) = \iiint \limits_T G(\bm{r}, \bm{r}_0)f(\bm{r})\d V
			- \dfrac{1}{\alpha} \iint \limits_\Sigma G(\bm{r}, \bm{r}_0) \phi(\bm{r})\d S	
	\end{align*}
\section{Miscellaneous}
	\subsection{Legendre Polynomial Integral}
		\begin{align*}
			&\int \limits^1_0 P_l(x)\d x
			= \left\{\begin{aligned}
				&1\, ,\quad l=0\\
				&\dfrac{1}{2}\, ,\quad l=1\\
				&0\, ,\quad l = 2n (n \geq 1)\\
				&(-1)^n\dfrac{(2n-1)!!}{(2n+1)!!}\, ,\quad l=2n+1 (n \geq 1)
			\end{aligned}\right.\\
			&\int \limits^1_0 xP_l(x)\d x
			= \left\{\begin{aligned}
				&\dfrac{1}{2}\, ,\quad l=0\\
				&\dfrac{1}{3}\, ,\quad l=1\\
				&(-1)^{n+1}\dfrac{1}{2n-1}\dfrac{(2n-1)!!}{(2n+2)!!}\, ,\quad l=2n (n \geq 1)\\
				&0\, ,\quad l = 2n+1 (n \geq 1)\\
			\end{aligned}\right.\\
			&\int \limits^1_0 x^2P_l(x)\d x
			= \left\{\begin{aligned}
				&\dfrac{1}{3}\, ,\quad l=0\\
				&\dfrac{1}{4}\, ,\quad l=1\\
				&\dfrac{2}{15}\, ,\quad l=2\\
				&\dfrac{1}{12}\, ,\quad l=3\\
				&0\, ,\quad l = 2n (n \geq 2)\\
				&(-1)^{n+1}\dfrac{(2n-3)!!}{(2n+4)!!}\, ,\quad l=2n+1 (n \geq 2)\\
			\end{aligned}\right.\\
		\end{align*}
	
	\subsection{Bessel Function Integral}
		\begin{align*}
			&\int J_1(x)\d x = -J_0(x) + C\\
			&\int x J_0(x)\d x = -xJ_1(x) + C\\
			&\int x J_2(x)\d x = -xJ_1(x) - 2 J_0(x) + C 
		\end{align*}
	\subsection{Laplace Transform}
			\begin{align*}
				\text{definition }\bar{f}(p) &= \int_{0}^{\infty}f(t)e^{-pt}\d t\\
				\L[f'(t)] &= p\bar{f}(p) - f(0)\\
				\L[\int^t_0f(t)\d t] &= \dfrac{1}{p}\bar{f}(p)\\
				\L[f(at)] &= \dfrac{1}{a}\bar{f}\left(\dfrac{p}{a}\right)\\
				\L[f(t-t_0)] &= e^{-p t_0}\bar{f}(p)\\
				\L[e^{-\lambda t}f(t)] &= f(p + \lambda)\\
				\L[f_1(t)*f_2(t)] &= \bar{f}_1(p) \bar{f}_2(p), \\
				f_1(t)*f_2(t) &= \int_{0}^{\infty}f_1(\tau)f_2(t-\tau)\d\tau
			\end{align*}
			\begin{align*}
				\L[1] &= \dfrac{1}{p}\\
				\L[t^n] &= \dfrac{n!}{p^{n+1}}\\
				\L[e^{st}] &= \dfrac{1}{p-s}\\
				\L[t^nf(t)] &= (-1)^n \dfrac{\d^n}{\d p^n} \bar{f}(p)\\
				\L[\sin\omega t] &= \dfrac{\omega}{p^2 + \omega^2}\\
				\L[\cos\omega t] &= \dfrac{p}{p^2 + \omega^2}
			\end{align*}

	\subsection{Gamma Function}
		\begin{align*}
			&\Gamma(x) = \int\limits^\infty_0 e^{-t} t^{x-1}\d t,\quad\Gamma(1) = 1,\quad\Gamma(\dfrac{1}{2}) = \sqrt{\pi}\\
			&\Gamma(x+1) = x\Gamma(x),\quad\Gamma(n + 1) = n!,\quad\Gamma(n+\dfrac{1}{2}) = n!\sqrt{\pi}\\
		\end{align*}
\begin{table*}[h]
	\centering
	\begin{tabular}{|c|c|c|c|}
		\hline
		equations & Spherical coord & \multicolumn{2}{c|}{Cylinder coord}\\ \hline
		\multirow{3}{*}{
			\begin{tabular}[c]{@{}c@{}}
				Laplace eq\\
				$\Delta u = 0$
			\end{tabular}
		} & 
		\multirow{3}{*}{
			\begin{tabular}[c]{@{}c@{}}
				$\Phi_m(\phi) = 
				\left\{\begin{aligned}
					\cos m\phi\\
					\sin m\phi
				\end{aligned}\right\}$
				\\
				$R_l(r) = 
				\left\{\begin{aligned}
					&r^l\\
					1/&r^{l+1}
				\end{aligned}\right\}$'
				\\
				$l$th order Associated Legendre eq:
				\\
				$\Theta_{m,l}(\theta) = \{P^m_l(\cos\theta)\}$\\
			\end{tabular}
		} & 
		\multicolumn{2}{c|}{
			$\Phi_m(\phi) = 
			\left\{\begin{aligned}
				\cos m\phi\\
				\sin m\phi
			\end{aligned}\right\}$}
		\\ \cline{3-4}
		&	&	
			\begin{tabular}[c]{@{}c@{}}
				When BC H on the side($R(\rho)$)
				\\
				$(\mu>0)$
				\\
				$Z_\mu(z) = 
				\left\{\begin{aligned}
					e^{\sqrt{\mu}z}\\
					e^{-\sqrt{\mu}z}
				\end{aligned}\right\}$
				\\
				$m$th order Bessel Function:
				\\
				$R_{m,\mu}(\rho) = 
				\left\{\begin{aligned}
					J_m(\sqrt{\mu}\rho)\\
					N_m(\sqrt{\mu}\rho)
				\end{aligned}\right\}$
			\end{tabular}
		&
			\begin{tabular}[c]{@{}c@{}}
				When BC H up and down($Z(z)$)
				\\
				$(\mu<0, h^2:=-\mu)$
				\\
				$Z_h(z) = 
				\left\{\begin{aligned}
					\cos hz\\
					\sin hz
				\end{aligned}\right\}$
				\\
				$m$th order Bessel Function with Im Arg:
				\\
				$R_{m,h}(\rho) = 
				\left\{\begin{aligned}
					I_m(h\rho)\\
					K_m(h\rho)
				\end{aligned}\right\}$
			\end{tabular}
		\\ \cline{3-4}
			&	&
		\multicolumn{2}{c|}{
			\begin{tabular}[c]{@{}c@{}}
				Always consider
				\\
				$(\mu=0, h^2:=-\mu = 0)$
				\\
				$Z_0(z) = 
				\left\{\begin{aligned}
					1\\
					z
				\end{aligned}\right\}$
				\\
				$R_0(\rho) = 
				\left\{\begin{aligned}
					1\\
					\ln\rho
				\end{aligned}\right\}, 
				R_m(\rho) = 
				\left\{\begin{aligned}
					\rho^m\\
					\rho^{-m}
				\end{aligned}\right\} (m\neq 0)$
			\end{tabular}
		} \\ \hline
		
		\begin{tabular}[c]{@{}c@{}}
			Wave eq\\
			$u_{tt}-a^2\Delta u=0$
		\end{tabular}
		
		& \multicolumn{3}{c|}{
			\begin{tabular}[c]{@{}c@{}}
			$T_0(t) = 
			\left\{\begin{aligned}
				1\\
				t
			\end{aligned}\right\}$;
			$T_k(t) = 
			\left\{\begin{aligned}
				\cos kat\\
				\sin kat
			\end{aligned}\right\}$
			or
			$T_k(t) = 
			\left\{\begin{aligned}
				e^{ikat}\\
				e^{-ikat}
			\end{aligned}\right\}(k\neq 0)$
			\\
			$\Delta v+k^2v=0$
			\end{tabular}
		} \\ \hline
		
		\begin{tabular}[c]{@{}c@{}}
			Transport eq\\
			$u_{t}-a^2\Delta u=0$
		\end{tabular}

		& \multicolumn{3}{c|}{
			\begin{tabular}[c]{@{}c@{}}
				$T_k(t)=e^{-k^2a^2t}$
				\\
				$\Delta v+k^2v=0$
				\end{tabular}
		} \\ \hline
		
		\begin{tabular}[c]{@{}c@{}}
			Helmholz eq\\
			$\Delta v+k^2v=0$
		\end{tabular}
		
		&

		\begin{tabular}[c]{@{}c@{}}
			$\Phi_m(\phi) = 
			\left\{\begin{aligned}
				\cos m\phi\\
				\sin m\phi
			\end{aligned}\right\}$
			\\
			$l$th order Associated Legendre eq:
			\\
			$\Theta_{m,l}(\theta) = \{P^m_l(\cos\theta)\}$
			\\
			$l$th order Spherical Bessel Function: 
			\\
			$R_{l,k}(r) = 
			\left\{\begin{aligned}
				j_l(kr)\\
				n_l(kr)
			\end{aligned}\right\}(k\neq 0)$,
			\\
			$R_l(r) = \left\{\begin{aligned}
				&r^l\\
				1/&r^{l+1}
			\end{aligned}\right\}(k = 0)$
		\end{tabular}

		& \multicolumn{2}{c|}{
			
		\begin{tabular}[c]{@{}c@{}}
			$\Phi_m(\phi) = 
			\left\{\begin{aligned}
				\cos m\phi\\
				\sin m\phi
			\end{aligned}\right\}$
			\\
			$Z_h(z) = 
			\left\{\begin{aligned}
				\cos hz\\
				\sin hz
			\end{aligned}\right\}(h\neq 0),
			Z_0(z) = 
			\left\{\begin{aligned}
				1\\
				z
			\end{aligned}\right\}(h=0)$
			\\
			$m$th order Bessel Function:
			\\
			$R_{m,k,h}(\rho) = 
			\left\{\begin{aligned}
				J_m(\sqrt{k^2-h^2}\rho)\\
				N_m(\sqrt{k^2-h^2}\rho)
			\end{aligned}\right\}$,
			\\
			if $(k=h=0)$
			\\
			$R_0(\rho) = 
			\left\{\begin{aligned}
				1\\
				\ln\rho
			\end{aligned}\right\}, 
			R_m(\rho) = 
			\left\{\begin{aligned}
				\rho^m\\
				\rho^{-m}
			\end{aligned}\right\} (m\neq 0)$
		\end{tabular}
		
		} \\ \hline
	\end{tabular}
\end{table*}

\end{document}
